src/impl/TLS13.Record.Framing.fsti
@@ -36,3 +36,20 @@ fn encode_inner_plaintext_no_padding
                         (SZ.v plain_len)
                         (SZ.v out_len)
                         content_type)
+
+fn decode_inner_plaintext_no_padding
+  (inner: array U8.t)
+  (inner_len: SZ.t)
+  (content_type_out: array U8.t)
+  (content_type_out_len: SZ.t)
+  requires pts_to inner 'inner_bytes **
+           pts_to content_type_out 'old_content_type **
+           pure (B.length 'inner_bytes == SZ.v inner_len /\
+                 B.length 'old_content_type == SZ.v content_type_out_len /\
+                 SZ.v inner_len > 0 /\
+                 SZ.v content_type_out_len == 1)
+  returns payload_len: (p:SZ.t{SZ.v p + 1 == SZ.v inner_len})
+  ensures exists* content_type_bytes.
+          pts_to inner 'inner_bytes **
+          pts_to content_type_out content_type_bytes **
+          pure (B.length content_type_bytes == 1)
